Very interesting state for three that is great for tutorial

Test/tutorial/LRU_cache/three.dfy
@@ -4,28 +4,28 @@ datatype Outcome<T> =
 
 datatype entry<T(!new,==)> = Entry(key: nat,value: T)
 	
-datatype Option<T> =
-	| Some(value: T)
-	| None
+datatype Ref<T> =
+	| Alloc(deref: T)
+	| Null
 
 class Item<T(!new,==)> {
 	
-	var more_recently_used: Option<Item<T>>
-	var less_recently_used: Option<Item<T>>
+	var more_recently_used: Ref<Item<T>>
+	var less_recently_used: Ref<Item<T>>
 	const key: nat
 	var value: T
 
 	constructor(key: nat, value: T)
 		ensures this.key == key
 		ensures this.value == value
-		ensures this.more_recently_used == None
-		ensures this.less_recently_used == None
+		ensures this.more_recently_used == Null
+		ensures this.less_recently_used == Null
 	{
 
 		this.key := key;
 		this.value := value;
-		more_recently_used := None;
-		less_recently_used := None;
+		more_recently_used := Null;
+		less_recently_used := Null;
 
 	}
 	
@@ -39,32 +39,64 @@ class LRUCache<T(!new,==)> {
 
 	const cache_size: nat
 		
-	var cache_head: Option<Item<T>>
-	var cache_tail: Option<Item<T>>
+	var cache_head: Ref<Item<T>>
+	var cache_tail: Ref<Item<T>>
 	var cache: map<nat,Item<T>>
 
 	predicate Invariant()
 		reads this, Repr
 	{
-		&& (forall key: nat :: key in cache ==> key in storage)
+
+		// Dynamic frame properties
 		&& (forall key: nat :: key in cache ==> cache[key] in Repr)
+		&& (cache_head.Alloc? ==> cache_head.deref in Repr)
+		&& (cache_tail.Alloc? ==> cache_tail.deref in Repr)
+		&& (forall i: Item :: i in Repr ==> i.more_recently_used.Null? || i.more_recently_used.deref in Repr)
+		&& (forall i: Item :: i in Repr ==> i.less_recently_used.Null? || i.less_recently_used.deref in Repr)
+		
+		// Functional properties
+		&& (forall key: nat :: key in cache ==> key in storage)
 		&& (forall key: nat :: key in cache ==> cache[key].key == key)
 		&& (forall key: nat :: key in cache ==> cache[key].value == storage[key])
-		&& (cache_head.Some? ==> cache_head.value in Repr)
-		&& (cache_tail.Some? ==> cache_tail.value in Repr)
-		&& (forall i: Item :: i in Repr ==> i.more_recently_used.None? || i.more_recently_used.value in Repr)
-		&& (forall i: Item :: i in Repr ==> i.less_recently_used.None? || i.less_recently_used.value in Repr)
 		&& (forall key, key': nat :: key in cache && key' in cache && key != key' ==> cache[key] != cache[key'])
-		&& (cache_head.Some? ==> cache_head.value.more_recently_used.None?)
-		&& (cache_tail.Some? ==> cache_tail.value.less_recently_used.None?)
-		&& (forall i: Item :: i in Repr && Some(i) != cache_head ==> i.more_recently_used.Some?)
-		&& (forall i: Item :: i in Repr && Some(i) != cache_tail ==> i.less_recently_used.Some?)
-		&& (forall i: Item :: i in Repr && i.more_recently_used.Some? ==> i.more_recently_used.value.less_recently_used == Some(i))
-		&& (forall i: Item :: i in Repr && i.less_recently_used.Some? ==> i.less_recently_used.value.more_recently_used == Some(i))
-		&& (|cache| == 0 ==> cache_head == cache_tail == None)
-		&& (|cache| == 1 ==> cache_head == cache_tail)
-		&& (|cache| >= 1 ==> cache_head.Some? && cache_tail.Some?)
-		&& (|cache| >= 2 <==> cache_head != cache_tail)
+
+		// Structural properties
+		&& (|cache| == 0 <==> Repr == {})
+		&& (|cache| == 0 <==> cache_head == cache_tail == Null)
+		&& (|cache| == 1 ==> (cache_head == cache_tail && cache_head.Alloc?))
+		&& (cache_head.Alloc? ==> cache_head.deref.more_recently_used.Null?)
+		&& (cache_tail.Alloc? ==> cache_tail.deref.less_recently_used.Null?)
+		&& (|cache| == 1 ==> Repr == {cache_head.deref})
+		&& (|cache| >= 1 <==> cache_head.Alloc? && cache_tail.Alloc?)
+		&& (|cache| >= 2 ==> cache_head != cache_tail)
+		&& (|cache| >= 2 ==> cache_head.deref.less_recently_used.Alloc?)
+		&& (|cache| >= 2 ==> cache_tail.deref.more_recently_used.Alloc?)
+		
+		// && |old(cache)| <= |cache| that would be nice but require twostate and then it "spreads"
+
+		
+		
+		
+		
+
+		&& (forall i: Item :: i in Repr ==> (i.more_recently_used.Alloc? && i.less_recently_used.Alloc? <==> Alloc(i) != cache_head && Alloc(i) != cache_tail))
+		
+
+		//&& (|cache| == 1 ==> (cache_head == cache_tail && cache_head.Alloc?))
+		//&& (|cache| == 1 <== (cache_head == cache_tail && cache_head.Alloc?))
+		//&& (|cache| >= 2 ==> cache_head != cache_tail)
+		//&& (|cache| >= 2 <== cache_head != cache_tail)
+		//&& (|cache| >= 2 <==> cache_head != cache_tail)
+		
+		
+		//&& (cache_head.Some? ==> cache_head.value.more_recently_used.None?)
+		//&& (cache_tail.Some? ==> cache_tail.value.less_recently_used.None?)
+		//&& (forall i: Item :: i in Repr && Some(i) != cache_head ==> i.more_recently_used.Some?)
+		// && (forall i: Item :: i in Repr && Some(i) != cache_tail ==> i.less_recently_used.Some?)
+		//&& (forall i: Item :: i in Repr && i.more_recently_used.Some? ==> i.more_recently_used.value.less_recently_used == Some(i))
+		//&& (forall i: Item :: i in Repr && i.less_recently_used.Some? ==> i.less_recently_used.value.more_recently_used == Some(i))
+
+		//&& (|cache| >= 2 <==> cache_head != cache_tail)
 
 	}
 	
@@ -74,48 +106,53 @@ class LRUCache<T(!new,==)> {
 	{
 		cache_size := size;
 		storage := map[];
-		cache_head := None;
-		cache_tail := None;
+		cache_head := Null;
+		cache_tail := Null;
 		cache := map[];
 		Repr := {};
 	}
 
-	method promote(key: nat)
-		modifies this, Repr
-		requires key in cache
-		requires Invariant()
-		ensures Invariant()
-		//ensures cache_head.Some? ==> cache_head.value.key == key
-	{
-		var item := cache[key];
-		if |cache| >= 2 {
-			if item.more_recently_used.Some? {
-				if item.less_recently_used.Some? {
-					assert cache_tail.value.less_recently_used.None?;
-					item.more_recently_used.value.less_recently_used := item.less_recently_used;
-					//assert cache_tail.value.less_recently_used.None?;
-					item.less_recently_used.value.more_recently_used := item.more_recently_used;
-					cache_head.value.less_recently_used := Some(item);
-					item.less_recently_used := cache_head;
-					item.more_recently_used := None;
-					cache_head := Some(item);
-					//assume false;
-				} else {
+	// method promote(key: nat)
+	// 	modifies this, Repr
+	// 	requires key in cache
+	// 	requires Invariant()
+	// 	ensures Invariant()
+	// 	//ensures cache_head.Some? ==> cache_head.value.key == key
+	// {
+	// 	var item := cache[key];
+	// 	if |cache| >= 2 {
+	// 		if item.more_recently_used.Alloc? {
+	// 			if item.less_recently_used.Alloc? {
+	// 				assert (cache_tail.Alloc? ==> cache_tail.deref.less_recently_used.Null?);
+	// 				//assert (|cache| == 1 <== (cache_head == cache_tail && cache_head.Alloc?));
+	// 				item.more_recently_used.deref.less_recently_used := item.less_recently_used;
+	// 				item.less_recently_used.deref.more_recently_used := item.more_recently_used;
+	// 				cache_head.deref.less_recently_used := Alloc(item);
+	// 				item.less_recently_used := cache_head;
+	// 				item.more_recently_used := Null;
+	// 				cache_head := Alloc(item);
+
+	// 				assume (cache_tail.Alloc? ==> cache_tail.deref.less_recently_used.Null?);
+	// 				//assume false;
+	// 			} else {
+	// 				//assert |cache| >= 2 ==> cache_head != cache_tail;
+	// 				cache_tail := item.more_recently_used;
+	// 				cache_tail.deref.less_recently_used := Null;
+	// 				//item.more_recently_used.value.less_recently_used := None;
+	// 				cache_head.deref.less_recently_used := Alloc(item);
+	// 				var old_cache_head := cache_head;
+	// 				cache_head := Alloc(item);
+	// 				cache_head.deref.less_recently_used := old_cache_head;
+	// 				cache_head.deref.more_recently_used := Null;
 					
-					//assert |cache| >= 2 ==> cache_head != cache_tail;
-					cache_tail := item.more_recently_used;
-					cache_tail.value.less_recently_used := None;
-					//item.more_recently_used.value.less_recently_used := None;
-					cache_head.value.less_recently_used := Some(item);
-					var old_cache_head := cache_head;
-					cache_head := Some(item);
-					cache_head.value.less_recently_used := old_cache_head;
-					cache_head.value.more_recently_used := None;
-					assume false;
-				}
-			}
-		}
-	}
+	// 				assume false;
+	// 			}
+	// 		}
+	// 	}
+	// 	// useful for debugging
+	// 	assert |old(cache)| == |cache|;
+	// 	assert |old(Repr)| == |Repr|;
+	// }
 	
 	method put_cache(key: nat, value: T)
 		modifies this, Repr
@@ -126,18 +163,60 @@ class LRUCache<T(!new,==)> {
 		ensures Invariant()
 	{
 
-		var item: Item := new Item(key,value);
-		Repr := Repr + {item};
-		
 		if |cache| == 0 {
+			var item: Item := new Item(key,value);
+			Repr := Repr + {item};
 			cache := cache[key := item];
-			cache_head := Some(item);
-			cache_tail := Some(item);
+			cache_head := Alloc(item);
+			cache_tail := Alloc(item);
+		} else if |cache| == 1 {
+			
+			var item: Item := new Item(key,value);
+			cache := cache[key := item];
+			
+			Repr := Repr + {item};
+			cache_head := Alloc(item);
+			cache_head.deref.less_recently_used := cache_tail;
+			cache_tail.deref.more_recently_used := cache_head;
+
+			//assert cache_head.deref.more_recently_used.Null?;
+			//assert cache_tail.deref.less_recently_used.Null?;
+			
+			//assert (forall i: Item :: i in Repr ==> (i.more_recently_used.Alloc? && i.less_recently_used.Alloc? ==> Alloc(i) != cache_head && Alloc(i) != cache_tail));
+			//assert (forall i: Item :: i in Repr ==> (i.more_recently_used.Alloc? && i.less_recently_used.Alloc? <== Alloc(i) != cache_head && Alloc(i) != cache_tail));
+			
+			
 		} else {
-			item.less_recently_used := cache_head;
+			
+			var item: Item := new Item(key,value);
 			cache := cache[key := item];
-			cache_head.value.more_recently_used := Some(item);
-			cache_head := Some(item);
+			
+			assert (forall i: Item :: i in Repr ==> (i.more_recently_used.Alloc? && i.less_recently_used.Alloc? <==> Alloc(i) != cache_head && Alloc(i) != cache_tail));
+			assert cache_head != cache_tail;
+			Repr := Repr + {item};
+			var old_cache_head := cache_head;
+			assert old_cache_head != cache_tail;
+			item.less_recently_used := cache_head;
+			old_cache_head.deref.more_recently_used := Alloc(item);
+			cache_head := Alloc(item);
+
+			assert (forall i: Item :: i in Repr ==> (i.more_recently_used.Alloc? && i.less_recently_used.Alloc? ==> Alloc(i) != cache_head && Alloc(i) != cache_tail));
+			
+			assert (forall i: Item :: i in Repr ==> (i.more_recently_used.Alloc? && i.less_recently_used.Alloc? <== Alloc(i) != cache_head && Alloc(i) != cache_tail)) by {
+				forall i: Item ensures i in Repr ==> (i.more_recently_used.Alloc? && i.less_recently_used.Alloc? <== Alloc(i) != cache_head && Alloc(i) != cache_tail) {
+					if i in Repr {
+						if  Alloc(i) != cache_head && Alloc(i) != cache_tail {
+							if Alloc(i) == old_cache_head {
+								//assume i.more_recently_used.Alloc? && i.less_recently_used.Alloc?;
+							} else {
+								assert true;
+							}
+						}
+					}
+				}
+			}
+			
+			//assume false;
 		}
 		
 		//assume false;
@@ -167,6 +246,8 @@ class LRUCache<T(!new,==)> {
 			
 		
 	}
+
+	// Step 1: put, get, no promotion, no eviction
 	
 	method get(key: nat) returns (result: Outcome<T>)
 		modifies this, Repr
@@ -175,7 +256,7 @@ class LRUCache<T(!new,==)> {
 	{
 		if key in cache {
 			result := Success(cache[key].value);
-			promote(key);
+			//promote(key);
 		} else if key in storage {
 			var value: T := storage[key];
 			result := Success(value);
@@ -190,27 +271,10 @@ class LRUCache<T(!new,==)> {
 		requires Invariant()
 		ensures Invariant()
 	{
-		//assert forall key': nat :: key' in cache ==> cache[key'].value == storage[key'];
-
 		storage := storage[key := value];
-
-		//assert forall key': nat :: key' in cache && key' != key ==> cache[key'].value == storage[key'];
-		//assert forall key': nat :: key' in cache ==> cache[key'].value == old(storage)[key'];
-
 		if key in cache {
 			cache[key].value := value;
 			assert cache[key].value == storage[key];
-			// assert forall key': nat :: key' != key && key' in cache ==> cache[key'].value == storage[key'] by {
-			// 	forall key': nat ensures key' != key && key' in cache ==> cache[key'].value == storage[key'] {
-			// 		if key' != key && key' in cache {
-			// 			assert cache[key'].value == old(cache)[key'].value;
-			// 			assert storage[key'] == old(storage)[key'];
-			// 			// Aliasing!
-			// 			assert old(cache)[key'].value == old(cache[key'].value);
-			// 			assert old(cache[key'].value) == old(storage)[key'];
-			// 		}
-			// 	}
-			// }
 		}
 	}
 
